Relico/Tests/MultiStorePayloadSelectionCompatibility.lean
@@ -1,0 +1,231 @@
+import Relico.Correctness.MultiStorePayloadSelectionCompatibility
+
+set_option autoImplicit false
+
+namespace Relico
+namespace Tests
+namespace MultiStorePayloadSelectionCompatibility
+
+theorem empty_compatible
+    (messageServers :
+      List DTR.MultiStorePayloadMessageServer) :
+    Correctness.MultiStorePayloadSelectionCompatible
+      messageServers
+      []
+      [] :=
+
+  Correctness.multiStorePayloadSelectionCompatible_nil
+    messageServers
+
+theorem same_microstep_pair_compatible
+    {messageServers :
+      List DTR.MultiStorePayloadMessageServer}
+    {sourceLeft sourceRight :
+      DTR.PendingMessage}
+    {targetLeft targetRight :
+      LF.PendingAction}
+    (hLeft :
+      Correctness.PendingCorresponds
+        sourceLeft
+        targetLeft)
+    (hRight :
+      Correctness.PendingCorresponds
+        sourceRight
+        targetRight)
+    (hSameMicrostep :
+      targetLeft.tag.microstep =
+        targetRight.tag.microstep) :
+    Correctness.MultiStorePayloadBasePairSelectionCompatible
+      messageServers
+      sourceLeft
+      sourceRight
+      targetLeft
+      targetRight :=
+
+  Correctness.multiStorePayloadBasePairSelectionCompatible_of_sameMicrostep
+      hLeft
+      hRight
+      hSameMicrostep
+
+theorem earlier_microstep_pair_compatible
+    {messageServers :
+      List DTR.MultiStorePayloadMessageServer}
+    {sourceLeft sourceRight :
+      DTR.PendingMessage}
+    {targetLeft targetRight :
+      LF.PendingAction}
+    (hLeft :
+      Correctness.PendingCorresponds
+        sourceLeft
+        targetLeft)
+    (hRight :
+      Correctness.PendingCorresponds
+        sourceRight
+        targetRight)
+    (hMicrostep :
+      targetLeft.tag.microstep <
+        targetRight.tag.microstep)
+    (hPriority :
+      Correctness.MultiStorePayloadBaseStrictPriorityPrecedes
+        messageServers
+        sourceLeft.name
+        sourceRight.name) :
+    Correctness.MultiStorePayloadBasePairSelectionCompatible
+      messageServers
+      sourceLeft
+      sourceRight
+      targetLeft
+      targetRight :=
+
+  Correctness.multiStorePayloadBasePairSelectionCompatible_of_leftEarlier
+      hLeft
+      hRight
+      hMicrostep
+      hPriority
+
+theorem earlier_microstep_recovers_priority
+    {messageServers :
+      List DTR.MultiStorePayloadMessageServer}
+    {sourceLeft sourceRight :
+      DTR.PendingMessage}
+    {targetLeft targetRight :
+      LF.PendingAction}
+    (hCompatible :
+      Correctness.MultiStorePayloadBasePairSelectionCompatible
+        messageServers
+        sourceLeft
+        sourceRight
+        targetLeft
+        targetRight)
+    (hSameTime :
+      sourceLeft.arrivalTime =
+        sourceRight.arrivalTime)
+    (hEarlier :
+      targetLeft.tag.microstep <
+        targetRight.tag.microstep) :
+    Correctness.MultiStorePayloadBaseStrictPriorityPrecedes
+      messageServers
+      sourceLeft.name
+      sourceRight.name :=
+
+  hCompatible.strictPriority_of_leftEarlier
+    hSameTime
+    hEarlier
+
+theorem payload_projects_base
+    {messageServers :
+      List DTR.MultiStorePayloadMessageServer}
+    {sourceBag :
+      DTR.MessageBag}
+    {targetQueue :
+      LF.ActionQueue}
+    (hCompatible :
+      Correctness.MultiStorePayloadSelectionCompatible
+        messageServers
+        sourceBag
+        targetQueue) :
+    Correctness.MultiStorePayloadBaseSelectionCompatible
+      messageServers
+      sourceBag
+      targetQueue :=
+
+  hCompatible.toSelectionCompatible
+
+theorem payload_projects_exact_bag
+    {messageServers :
+      List DTR.MultiStorePayloadMessageServer}
+    {sourceBag :
+      DTR.MessageBag}
+    {targetQueue :
+      LF.ActionQueue}
+    (hCompatible :
+      Correctness.MultiStorePayloadSelectionCompatible
+        messageServers
+        sourceBag
+        targetQueue) :
+    Correctness.MultiStorePayloadBagQueueCorresponds
+      sourceBag
+      targetQueue :=
+
+  hCompatible.toPayloadBagQueueCorresponds
+
+theorem aligned_occurrence_preserves_payload
+    {messageServers :
+      List DTR.MultiStorePayloadMessageServer}
+    {sourceRepresentative :
+      DTR.MessageBag}
+    {targetRepresentative :
+      LF.ActionQueue}
+    {sourceMessage :
+      DTR.PendingMessage}
+    {targetAction :
+      LF.PendingAction}
+    (hCompatible :
+      Correctness.MultiStorePayloadOrderedSelectionCompatible
+        messageServers
+        sourceRepresentative
+        targetRepresentative)
+    (hAligned :
+      Correctness.MultiStorePayloadBaseAlignedOccurrence
+        sourceMessage
+        targetAction
+        sourceRepresentative
+        targetRepresentative) :
+    Correctness.PendingPayloadCorresponds
+      sourceMessage
+      targetAction :=
+
+  hCompatible.alignedPayload
+    hAligned
+
+theorem source_permutation_preserves_compatibility
+    {messageServers :
+      List DTR.MultiStorePayloadMessageServer}
+    {sourceLeft sourceRight :
+      DTR.MessageBag}
+    {targetQueue :
+      LF.ActionQueue}
+    (hPermutation :
+      sourceLeft.Perm
+        sourceRight)
+    (hCompatible :
+      Correctness.MultiStorePayloadSelectionCompatible
+        messageServers
+        sourceRight
+        targetQueue) :
+    Correctness.MultiStorePayloadSelectionCompatible
+      messageServers
+      sourceLeft
+      targetQueue :=
+
+  Correctness.MultiStorePayloadSelectionCompatible.perm_source
+    hPermutation
+    hCompatible
+
+theorem target_permutation_preserves_compatibility
+    {messageServers :
+      List DTR.MultiStorePayloadMessageServer}
+    {sourceBag :
+      DTR.MessageBag}
+    {targetLeft targetRight :
+      LF.ActionQueue}
+    (hPermutation :
+      targetLeft.Perm
+        targetRight)
+    (hCompatible :
+      Correctness.MultiStorePayloadSelectionCompatible
+        messageServers
+        sourceBag
+        targetRight) :
+    Correctness.MultiStorePayloadSelectionCompatible
+      messageServers
+      sourceBag
+      targetLeft :=
+
+  Correctness.MultiStorePayloadSelectionCompatible.perm_target
+    hPermutation
+    hCompatible
+
+end MultiStorePayloadSelectionCompatibility
+end Tests
+end Relico
